\documentclass[a4paper]{article}

\usepackage[english]{babel}
\usepackage[utf8x]{inputenc}
\usepackage{amsmath}
\usepackage{graphicx}

\title{MATH 542 Homework 8}
\author{Saket Choudhary\\skchoudh@usc.edu}

\begin{document}
\maketitle 
\subsection*{Problem 3a.2}
Consider $||\boldmath{Y}-\boldmath{X\beta}||^2$.  Since X is full rank $\hat{\beta} = (X'X)^{-1}X'Y$
This involves $\frac{||\boldmath{Y}-\boldmath{X\beta}||^2}{\partial \beta_i}=0$
Also $\hat{Y_i}=\beta_0+x_{i1}\beta_1 + \dots + x_{ip-1}\beta_{p-1} $
For $i=0$:
\begin{align*}
\frac{||\boldmath{Y}-\boldmath{X\beta}||^2}{\partial \beta_i}&=0\\
\frac{\sum( Y_i-(\beta_0+x_{i1}\beta_1 + \dots + x_{ip-1}\beta_{p-1} ) )^2 }{\partial \beta_0} &= 0\\
\sum( Y_i-(\beta_0+x_{i1}\beta_1 + \dots + x_{ip-1}\beta_{p-1} ) ) &= 0\\
\sum( Y_i-\hat{Y_i} ) &= 0\\
\end{align*}
\subsection*{Problem 3a.3}
\begin{align*}
\begin{pmatrix}Y_1\\Y_2\\Y_3
\end{pmatrix}&= \begin{pmatrix}1 &0\\ 2 & -1\\ 1 & 2\end{pmatrix}\begin{pmatrix}\theta\\ \phi \end{pmatrix}\\
\end{align*}
Thus $X=\begin{pmatrix}1 &0\\ 2 & -1\\ 1 & 22\end{pmatrix}$
$\beta=X'X$ and hence using R:
\begin{align*}
\theta = 0.167 Y_1 + 0.333 Y_2 + 0.167 Y_3\\
\phi = -0.2Y_2+0.4Y_3
\end{align*}
\subsection*{Problem 3a.4}
\begin{align*}
\begin{pmatrix}Y_1\\Y_2\\Y_3
\end{pmatrix}&= \begin{pmatrix}1 &-1 &1\\ 1 & 0 & -2\\ 1 & 1 &1\end{pmatrix}\begin{pmatrix}\beta_0\\ \beta_1 \\ \beta_2\end{pmatrix}\\
\end{align*}

\begin{align*}
\begin{pmatrix}\beta_0\\ \beta_1 \\ \beta_2\end{pmatrix}&= (X'X)^{-1}X'Y\\
\begin{pmatrix}\beta_0\\ \beta_1 \\ \beta_2\end{pmatrix}&= \begin{pmatrix}\frac{1}{3} & \frac{1}{3} & \frac{1}{3}\\ -0.5 & 0 & 0.5\\ \frac{1}{6} & -\frac{1}{3} & \frac{1}{6}\end{pmatrix}\begin{pmatrix}Y_1\\Y_2\\Y_3
\end{pmatrix}
\end{align*}
Consider $\beta_2=0$:


\begin{align*}
\begin{pmatrix}Y_1\\Y_2\\Y_3
\end{pmatrix}&= \begin{pmatrix}1 &-1 \\ 1 & 0 \\ 1 & 1\end{pmatrix}\begin{pmatrix}\beta_0\\ \beta_1 \\\end{pmatrix}\\
\end{align*}

Then using R:
\begin{align*}
\begin{pmatrix}\beta_0\\ \beta_1\end{pmatrix}&= (X'X)^{-1}X'Y\\
\begin{pmatrix}\beta_0\\ \beta_1\end{pmatrix}&= \begin{pmatrix}\frac{1}{3} & \frac{1}{3} & \frac{1}{3}\\ -0.5 & 0 & 0.5\\ \end{pmatrix}\begin{pmatrix}Y_1\\Y_2\\Y_3
\end{pmatrix}
\end{align*}

\subsection*{Problem 3a.7}
$\hat{Y} = X\hat{\beta} = PY$
\begin{align*}
\sum \hat{Y_i}(Y_i-\hat{Y_i}) &= \hat{Y'}(Y-\hat{Y'}\\
&= Y'P'(Y-PY)\\
&= Y'P(I_n-P)Y\\
&= Y'(P-P^2)Y\\
&=0\text{ Since P is idempotent}
\end{align*}
\subsection*{Problem 3b.3}
Consider $\bar{Y} = \frac{\sum_i Y_i}{n}$

$E[\bar{Y}] = \theta$ so $\bar{Y}$ is unbiased estimate.

Also using Rao's minimum variance lower bound, $\alpha'\beta$ is a minimum variance estimate for $\mathcal{N}(X\beta, \sigma^2)$, Thus $\bar{Y}$ is both unbiased and minimum variance.

\subsection*{Problem 3b.4}

\begin{align*}
Y_i &= \beta_0+\beta_1(x_{i1}-\bar{x_1}) + \beta_2(x_{i2}-\bar{x_2})+\epsilon_i\\
\begin{pmatrix}Y_1\\Y_2\\Y_3\\\vdots\\Y_n
\end{pmatrix}&= \begin{pmatrix} 1 & x_{11}-\bar{x_1} & x_{12}-\bar{x_2}\\
 1 & x_{21}-\bar{x_1} & x_{22}-\bar{x_2}\\
 \vdots 
 1 & x_{n1}-\bar{x_1} & x_{n2}-\bar{x_2}\\
\end{pmatrix}\begin{pmatrix}
\beta_0\\\beta_1\\\beta_2
\end{pmatrix}\\
X &= \begin{pmatrix} 1 & x_{11}-\bar{x_1} & x_{12}-\bar{x_2}\\
 1 & x_{21}-\bar{x_1} & x_{22}-\bar{x_2}\\
 \vdots 
 1 & x_{n1}-\bar{x_1} & x_{n2}-\bar{x_2}\\
\end{pmatrix}\\
X'X &= \begin{pmatrix}
n & \sum x_{i1}-n\bar{x_1} & \sum x_{i2} - n \bar{x_2}\\
\sum x_{i1}-n\bar{x_1} & \sum(x_{i1}-\bar{x_1})^2 & \sum (x_{i1}-\bar{x_1})(x_{i2}-\bar{x_2})\\
\sum x_{i2}-n\bar{x_2} & \sum (x_{i1}-\bar{x_1})(x_{i2}-\bar{x_2}) & \sum(x_{i2}-\bar{x_2})^2
\end{pmatrix}\\
& = \begin{pmatrix}
n & 0 & 0\\
0 & \sigma^2_{1} & r\sigma_1\sigma_2\\
0 & r\sigma_1\sigma_2 & \sigma_2^2
\end{pmatrix}\\ 
(X'X)^{-1} & = \frac{1}{\sigma_1^2\sigma_2^2(1-r^2)} \begin{pmatrix}
\frac{1}{n(\sigma_1^2\sigma_2^2(1-r^2))} & 0 & 0\\
0 & \sigma^2_{2} & r\sigma_1\sigma_2\\
0 & r\sigma_1\sigma_2 & \sigma_1^2
\end{pmatrix}\\ 
\end{align*}
Thus $Var(\beta_1) = \sigma^2 (X'X)^{-1} = \frac{\sigma^2 \sigma_2^2}{\sigma_1^2\sigma_2^2(1-r^2)} = \frac{\sigma^2}{\sigma_1^2(1-r^2)}$
\end{document}



