{
 "cells": [
  {
   "cell_type": "markdown",
   "metadata": {},
   "source": [
    "$$\\vec{x(t)} = \\begin{bmatrix} y(t) & \\dot{y(t)}\\end{bmatrix}^T$$\n",
    "\n",
    "\\begin{eqnarray*}\n",
    "m\\ddot{y} + c\\dot{y} + ky = bu\\\\\n",
    "\\ddot{y} + \\frac{c}{m}\\dot{y} + \\frac{k}{m}y = \\frac{b}{m}u\\\\\n",
    "\\ddot{y} = -\\frac{c}{m}\\dot{y} - \\frac{k}{m}y \\frac{b}{m}u\\\\\n",
    "\\end{eqnarray*}\n",
    "\n",
    "Thus we have:\n",
    "\n",
    "\\begin{eqnarray*}\n",
    "\\frac{dy}{dt} = \\dot{y}\\\\\n",
    "\\frac{d\\dot{y}}{dt} = -\\frac{c}{m}\\dot{y} - \\frac{k}{m}y + \\frac{b}{m}u\n",
    "\\end{eqnarray*}\n",
    "\n",
    "Thus,\n",
    "\\begin{eqnarray*}\n",
    "\\frac{d}{dt}\\begin{bmatrix} y(t+1) \\\\ \\dot{y}(t+1)  \\end{bmatrix} = \\begin{bmatrix} 0 & 1\\\\ -\\frac{k}{m} & -\\frac{c}{m} \\end{bmatrix} \\begin{bmatrix} y(t) \\\\ \\dot{y}(t) \\end{bmatrix} + \\begin{bmatrix} 0 \\\\ 1 \\end{bmatrix} u \\\\\n",
    "\\frac{d}{dt}\\vec{x}(t+1) = \\begin{bmatrix} 0 & 1\\\\ -\\frac{k}{m} & -\\frac{c}{m} \\end{bmatrix} \\vec{x}(t) + \\begin{bmatrix} 0 \\\\ 1 \\end{bmatrix} u(t) \\\\\n",
    "\\frac{d}{dt}\\vec{x}(t+1) = A \\vec{x}(t) + B u(t) \\\\\n",
    "\\end{eqnarray*}\n",
    "\n",
    "and the equation for measurement is given by in the interval $[k\\tau, (k+1)\\tau)$:\n",
    "\\begin{eqnarray*}\n",
    "y_k = y(k\\tau) + \\omega_k\\\\\n",
    "y_k = \\begin{bmatrix} 1 \\\\ 0\\end{bmatrix}  \\begin{bmatrix} y(t) \\\\ \\dot{y}(t) \\end{bmatrix} + \\omega_k \\\\\n",
    "y_k = \\begin{bmatrix} 1 \\\\ 0\\end{bmatrix} \\vec{x}_k + \\omega_k\n",
    "\\end{eqnarray*}\n",
    "\n",
    "In the domain $[k\\tau, (k+1)\\tau)$ we refformulate the equations as:\n",
    "\n",
    "\\begin{eqnarray*}\n",
    "\\frac{d}{dt}\\vec{x}(t+1) = A\\vec{x}(t) + Bu_t\\\\\n",
    "\\text{where } A = \\begin{bmatrix} 0 & 1\\\\ -\\frac{k}{m} & -\\frac{c}{m}\\end{bmatrix}\\\\\n",
    "\\text{and } B = \\begin{bmatrix} 0 \\\\ \\frac{b}{m} \\end{bmatrix} \n",
    "\\end{eqnarray*}\n",
    "\n",
    "And the obseration equation:\n",
    "\n",
    "\\begin{eqnarray*}\n",
    "y_k = C \\vec{x}_k + \\omega_k\\\\\n",
    "\\text{where } C = \\begin{bmatrix} 1 \\\\ 0\\end{bmatrix} \n",
    "\\end{eqnarray*}\n",
    "\n",
    "and the initial condition is given by:\n",
    "\\begin{eqnarray*}\n",
    "\\vec{x}(0) = \\begin{bmatrix} y(0) \\\\ \\dot{y}(0) \\end{bmatrix} = \\begin{bmatrix} y_0 + \\eta  \\\\ y_1 + \\varsigma \\end{bmatrix} = \\begin{bmatrix} y_0 \\\\ y_1 \\end{bmatrix} + \\begin{bmatrix} \\eta \\\\ \\varsigma \\end{bmatrix} = \\begin{bmatrix} y_0 \\\\ y_1 \\end{bmatrix} + \\vec{\\epsilon} \\\\\n",
    "\\text{where } \\vec{\\epsilon} = \\mathcal{N}(\\begin{bmatrix} 0 \\\\ 0 \\end{bmatrix}, Q)\\\\\n",
    "\\text{and } Q = \\begin{bmatrix} \\alpha^2 & 0 \\\\ 0 & \\beta^2 \\end{bmatrix} \\\\\n",
    "\\text{where } \\eta \\sim \\mathcal{N}(0, \\alpha^2) \\\\\n",
    "\\text{and } \\varsigma \\sim \\mathcal{N}(0, \\beta^2)\n",
    "\\end{eqnarray*}"
   ]
  },
  {
   "cell_type": "markdown",
   "metadata": {},
   "source": [
    "We now use variation of parameters on the interval $[k\\tau, (k+1)\\tau)$ t obtain:\n",
    "\n",
    "\\begin{eqnarray*}\n",
    "\\vec{x}_{k+1} = \\exp(A\\tau)x_{k} + \\int_{k\\tau}^{k\\tau+\\tau} \\exp(A(s-k\\tau)) B(s) u(s) ds\\\\\n",
    "\\vec{x}_{k+1} = \\exp(A\\tau)x_{k} + \\int_{k\\tau}^{k\\tau+\\tau} \\exp(A(s-k\\tau)) ds B(u_k + \\epsilon_k) \\\\\n",
    "\\vec{x}_{k+1} = \\exp(A\\tau)x_{k} + \\int_{0}^{\\tau} \\exp(As') ds' B(u_k + \\epsilon_k) \\ \\text{where } s'=s+k\\tau \\\\\n",
    "\\vec{x}_{k+1} = \\exp(A\\tau)x_{k} + \\int_{0}^{\\tau} \\exp(As') ds' B(u_k + \\epsilon_k) \\\\\n",
    "\\vec{x}_{k+1} = \\exp(A\\tau)x_{k} + A^{-1}(\\exp(A\\tau)-I)Bu_k + A^{-1}(\\exp(A\\tau)-I)B\\epsilon_k  \\\\\n",
    "\\end{eqnarray*}\n",
    "\n",
    "Now, \n",
    "\n",
    "\\begin{eqnarray*}\n",
    "\\exp(A\\tau) = I + \\frac{A\\tau}{1!} + \\frac{A^2\\tau^2}{2!} + \\frac{A^3\\tau^3}{3!} + \\dots \n",
    "\\end{eqnarray*}\n",
    "\n",
    "\n",
    "To formulate this as \n",
    "\n",
    "\\begin{eqnarray*}\n",
    "\\vec{x}_{k+1} = \\phi \\vec{x}_k + \\psi u_k + \\vec{v}_k\\\\\n",
    "\\phi = \\exp(A\\tau)\\\\\n",
    "\\psi = A^{-1}(\\exp(A\\tau)-I)B\\\\\n",
    "\\vec{v}_k =  A^{-1}(\\exp(A\\tau)-I)B\\epsilon_k = \\psi \\epsilon_k\n",
    "\\end{eqnarray*}\n",
    "\n",
    "And thus $\\vec{v}_k \\sim \\mathcal{N}(\\begin{bmatrix} 0 \\\\ 0 \\end{bmatrix}, V)$  where $V = \\sigma^2 \\psi \\psi^T$ where $\\psi_{2 \\times 1} = A^{-1}(\\exp(A\\tau)-I)B$"
   ]
  },
  {
   "cell_type": "markdown",
   "metadata": {
    "collapsed": true
   },
   "source": [
    "\\begin{eqnarray*}\n",
    "x_{k+1} = \\phi x_k + \\psi u_k + v_k\\\\\n",
    "\\bar{x}_{k+1} = \\phi \\bar{x_k} + \\psi u_k \\\\\n",
    "x_{k+1} - \\bar{x}_{k+1} = \\phi (x_k-\\bar{x_k}) + v_k\\\\\n",
    "\\end{eqnarray*}\n",
    "\n",
    "\\begin{align*}\n",
    "P_{k+1|k} &= E((x_{k+1} - \\bar{x}_{k+1})(x_{k+1} - \\bar{x}_{k+1})^T)\\\\\n",
    "&= E[(\\phi (x_k-\\bar{x_k}) + v_k)((x_k-\\bar{x_k})^T\\phi^T  + v_k^T)]\\\\\n",
    "&= E[\\phi(x_k-\\bar{x_k})(x_k-\\bar{x_k})^T\\phi^T + 2(x_k-\\bar{x_k})\\phi v_k + v_k v_k^T]\\\\\n",
    "&= \\phi P_{k|k} \\phi^T + V_k\n",
    "\\end{align*}"
   ]
  },
  {
   "cell_type": "markdown",
   "metadata": {},
   "source": [
    "### Prediction\n",
    "\n",
    "\\begin{align*}\n",
    "\\hat{x}_{k+1|k} &= \\phi \\hat{x}_k + \\psi u_k\\\\\n",
    "P_{k+1|k} &= \\phi P_{k|k} \\phi^T + V_k\n",
    "\\end{align*}"
   ]
  },
  {
   "cell_type": "markdown",
   "metadata": {},
   "source": [
    "### Observed/Measured\n",
    "\n",
    "\\begin{align*}\n",
    "x_{k+1|k} &= \\phi x_k + \\psi u_k + \\v_k\\\\\n",
    "y_{k+1|k} &= Cx_{k+1} + \\omega_k \n",
    "\\end{align*}"
   ]
  },
  {
   "cell_type": "markdown",
   "metadata": {},
   "source": [
    "### Update\n",
    "\n",
    "Assume update step to be linear combination of prediction and observation. We need to obtain $K_1, K_2$  such that the estimator is unbiased and is minimum variance estimate.\n",
    "\n",
    "\\begin{align*}\n",
    "\\hat{x}_{k+1|k+1} &= K_1 \\hat{x}_{k+1|k} + K_2 y_{k+1|k}\n",
    "\\end{align*}\n",
    "\n",
    "Define error $e_{k+1|k+1} = \\hat{x}_{k+1|k+1} - x_{k+1}$\n",
    "\n",
    "We look for unbiased estimator $E[e_{k+1|k+1}]=0$\n",
    "\n",
    "Thus,\n",
    "\n",
    "\\begin{align*}\n",
    "e_{k+1|k+1} &= \\hat{x}_{k+1|k+1} - x_{k+1}\\\\\n",
    "&= K_1 \\hat{x}_{k+1|k} +K_2(Cx_{k+1}+\\omega_{k+1}) - x_{k+1}\\\\\n",
    "&= K_1 \\hat{x}_{k+1|k} +(K_2C-I)x_{k+1} + K_2\\omega_{k+1}\\\\\n",
    "\\end{align*}\n",
    "\n",
    "Now, \n",
    "\n",
    "\\begin{align*}\n",
    "E[e_{k+1|k+1}] &=0\\\\\n",
    "\\implies K_1 &= I-K_2C\n",
    "\\end{align*}\n",
    "\n",
    "\n",
    "Thus, \n",
    "\\begin{align*}\n",
    "\\hat{x}_{k+1|k+1} &= (I-K_2C) \\hat{x}_{k+1|k} + K_2 y_{k+1|k}\\\\\n",
    "&= (I-K_2C) \\hat{x}_{k+1|k} + K_2(Cx_{k+1}+\\omega_{k+1})\\\\\n",
    "&= \\hat{x}_{k+1|k} + K_2C(x_{k+1}-\\hat{x}_{k+1|k}) + \\omega_{k+1}\n",
    "\\end{align*}\n",
    "\n",
    "Now, \n",
    "\\begin{align*}\n",
    "e_{k+1|k+1} &= \\hat{x}_{k+1|k+1} - x_{k+1}\\\\\n",
    "&= K_1 \\hat{x}_{k+1|k} +K_2(Cx_{k+1}+\\omega_{k+1}) - x_{k+1}\\\\\n",
    "&= (I-K_2C)\\hat{x}_{k+1|k} +(K_2C-I)x_{k+1} + K_2\\omega_{k+1}\\\\\n",
    "&= (I-K_2C)(\\hat{x}_{k+1|k}-x_{k+1}) + K_2\\omega_{k+1}\\\\\n",
    "&= (I-K_2C)e_{k+1|k} + K_2\\omega_{k+1}\\\\\n",
    "\\end{align*}\n",
    "\n",
    "where $e_{k+1|k} = \\hat{x}_{k+1|k}-x_{k+1}$\n",
    "Then,\n",
    "\\begin{align*}\n",
    "P_{k+1|k+1} &= E[e_{k+1|k+1}e_{k+1|k+1}^T] \\\\\n",
    "&= E[((I-K_2C)e_{k+1|k} + K_2\\omega_{k+1}) ((I-K_2C)e_{k+1|k} + K_2\\omega_{k+1})^T ]\\\\\n",
    "&= (I-K_2C)E[e_{k+1|k}^Te_{k+1|k}] (I-K_2C)^T + K_2E[\\omega_{k+1}\\omega_{k+1}^T]K_2^T\\\\\n",
    "&= (I-K_2C)P_{k+1|k}(I-K_2C)^T + K_2W_kK_2^T\\\\\n",
    "&= (P_{k+1|k} - K_2CP_{k+1|k}) (I-K_2C)^T+K_2W_kK_2^T\\\\\n",
    "&= P_{k+1|k} - K_2CP_{k+1|k} - P_{k+1|k}C^TK_2^T + K_2CP_{k+1|k}C^TK_2^T + K_2W_kK_2^T\\\\\n",
    "&= P_{k+1|k} - K_2CP_{k+1|k} - P_{k+1|k}C^TK_2^T + K_2( CP_{k+1|k}C^T + W_k)K_2^T\\\\\n",
    "\\end{align*}\n",
    "\n",
    "To minimize $\\frac{\\partial P_{k+1|k+1}}{\\partial K_2} =0$\n",
    "\n",
    "\\begin{align*}\n",
    "\\frac{\\partial P_{k+1|k+1}}{\\partial K_2}  = -2 P_{k+1|k}^TC + 2K_2(CP_{k+1|k}C^T + W_k) = 0\\\\\n",
    "\\implies K_2 = P_{k+1|k}^TC(CP_{k+1|k}C^T + W_k)^{-1}\n",
    "\\end{align*}\n"
   ]
  },
  {
   "cell_type": "markdown",
   "metadata": {},
   "source": [
    "\\begin{align*}\n",
    "\\hat{x}_{k+1|k+1} &= \\hat{x}_{k+1|k} + K_2(y_k - C\\hat{x}_{k+1|k})\\\\\n",
    "P_{k+1|k+1} &= P_{k+1|k} - K_2CP_{k+1|k} \\\\\n",
    "K_2 &= P_{k+1|k}^TC(CP_{k+1|k}C^T + W_k)^{-1}\n",
    "\\end{align*}"
   ]
  },
  {
   "cell_type": "code",
   "execution_count": null,
   "metadata": {
    "collapsed": true
   },
   "outputs": [],
   "source": []
  }
 ],
 "metadata": {
  "kernelspec": {
   "display_name": "Python 2",
   "language": "python",
   "name": "python2"
  },
  "language_info": {
   "codemirror_mode": {
    "name": "ipython",
    "version": 2
   },
   "file_extension": ".py",
   "mimetype": "text/x-python",
   "name": "python",
   "nbconvert_exporter": "python",
   "pygments_lexer": "ipython2",
   "version": "2.7.11"
  }
 },
 "nbformat": 4,
 "nbformat_minor": 0
}
